revm: links more instructions

CoqOfRust/alloy_primitives/bits/links/fixed_FixedBytes.v
@@ -1,25 +1,63 @@
 Require Import CoqOfRust.CoqOfRust.
 Require Import CoqOfRust.links.M.
+Require Import core.links.array.
 
 (* pub struct FixedBytes<const N: usize>(pub [u8; N]); *)
 Module FixedBytes.
-  Parameter t : Usize.t -> Set.
+  Record t {N : Usize.t} : Set := {
+    value : array.t U8.t N;
+  }.
+  Arguments t : clear implicits.
 
-  Parameter to_value : forall {N: Usize.t}, t N -> Value.t.
-
-  Global Instance IsLink (N: Usize.t): Link (t N) := {
+  Global Instance IsLink (N : Usize.t) : Link (t N) := {
     Φ := Ty.apply (Ty.path "alloy_primitives::bits::fixed::FixedBytes") [ φ N ] [];
-    φ := to_value;
+    φ x := Value.StructTuple "alloy_primitives::bits::fixed::FixedBytes" [φ N] [] [φ x.(value)];
   }.
 
-  Definition of_ty (N' : Value.t) (N: Usize.t) :
+  Definition of_ty (N' : Value.t) (N : Usize.t) :
     N' = φ N ->
     OfTy.t (Ty.apply (Ty.path "alloy_primitives::bits::fixed::FixedBytes") [ N' ] []).
   Proof.
     intros.
     eapply OfTy.Make with (A := t N).
-    subst.
-    reflexivity.
+    now subst.
   Defined.
-  Smpl Add eapply of_ty : of_ty.
+  Smpl Add unshelve eapply of_ty : of_ty.
+
+  Lemma of_value_with (N' : Value.t) (N : Usize.t) (value : array.t U8.t N) (value' : Value.t) :
+    N' = φ N ->
+    value' = φ value ->
+    Value.StructTuple "alloy_primitives::bits::fixed::FixedBytes" [N'] [] [value'] =
+    φ (Build_t N value).
+  Proof.
+    now intros; subst.
+  Qed.
+  Smpl Add unshelve eapply of_value_with : of_value.
+
+  Definition of_value (N' : Value.t) (N : Usize.t) (value' : Value.t) (value : array.t U8.t N) :
+    N' = φ N ->
+    value' = φ value ->
+    OfValue.t (Value.StructTuple "alloy_primitives::bits::fixed::FixedBytes" [N'] [] [value']).
+  Proof.
+    intros.
+    eapply OfValue.Make with (A := t N) (value := Build_t N value).
+    now subst.
+  Defined.
+  Smpl Add unshelve eapply of_value : of_value.
+
+  Module SubPointer.
+    Definition get_0 (N : Usize.t) : SubPointer.Runner.t (t N)
+      (Pointer.Index.StructTuple "alloy_primitives::bits::fixed::FixedBytes" 0) :=
+    {|
+      SubPointer.Runner.projection x := Some x.(value);
+      SubPointer.Runner.injection x y := Some (x <| value := y |>);
+    |}.
+
+    Lemma get_0_is_valid {N : Usize.t} :
+      SubPointer.Runner.Valid.t (get_0 N).
+    Proof.
+      now constructor.
+    Qed.
+    Smpl Add apply get_0_is_valid : run_sub_pointer.
+  End SubPointer.
 End FixedBytes.
