CoqOfRust/alloy_primitives/log/links/mod.v
@@ -1,5 +1,10 @@
 Require Import CoqOfRust.CoqOfRust.
 Require Import CoqOfRust.links.M.
+Require Import alloc.links.alloc.
+Require Import alloc.vec.links.mod.
+Require Import alloy_primitives.bits.links.address.
+Require Import alloy_primitives.bytes.links.mod.
+Require Import alloy_primitives.links.aliases.
 Require Import alloy_primitives.log.mod.
 
 (*
@@ -9,16 +14,106 @@ pub struct Log<T = LogData> {
 }
 *)
 Module Log.
-  Parameter t : Set.
+  Record t {T : Set} : Set := {
+    address : Address.t;
+    data : T;
+  }.
+  Arguments t : clear implicits.
 
-  Parameter to_value : t -> Value.t.
-
-  Global Instance IsLink : Link t := {
-    Φ := Ty.path "alloy_primitives::log::Log";
-    φ := to_value;
+  Global Instance IsLink (T : Set) `{Link T}: Link (t T) := {
+    Φ := Ty.apply (Ty.path "alloy_primitives::log::Log") [] [Φ T];
+    φ x :=
+      Value.StructRecord "alloy_primitives::log::Log" [] [Φ T] [
+        ("address", φ x.(address));
+        ("data", φ x.(data))
+      ];
   }.
 
-  Definition of_ty : OfTy.t (Ty.path "alloy_primitives::log::Log").
-  Proof. eapply OfTy.Make with (A := t); reflexivity. Defined.
-  Smpl Add apply of_ty : of_ty.
+  Definition of_ty T' :
+    OfTy.t T' ->
+    OfTy.t (Ty.apply (Ty.path "alloy_primitives::log::Log") [] [T']).
+  Proof.
+    intros [T].
+    eapply OfTy.Make with (A := t T).
+    now subst.
+  Defined.
+  Smpl Add unshelve eapply of_ty : of_ty.
+
+  Lemma of_value_with
+      (T : Set) `{Link T} T'
+      address address'
+      (data : T) data' :
+    T' = Φ T ->
+    address' = φ address ->
+    data' = φ data ->
+    Value.StructRecord "alloy_primitives::log::Log" [] [T'] [
+      ("address", address');
+      ("data", data')
+    ] = φ (Build_t T address data).
+  Proof.
+    intros.
+    now subst.
+  Qed.
+  Smpl Add unshelve eapply of_value_with : of_value.
 End Log.
+
+(*
+pub struct LogData {
+    topics: Vec<B256>,
+    pub data: Bytes,
+}
+*)
+Module LogData.
+  Record t : Set := {
+    topics : Vec.t aliases.U256.t Global.t;
+    data : Bytes.t;
+  }.
+
+
+  Global Instance IsLink : Link t := {
+    Φ := Ty.path "alloy_primitives::log::LogData";
+    φ x :=
+      Value.StructRecord "alloy_primitives::log::LogData" [] [] [
+        ("data", φ x.(data));
+        ("topics", φ x.(topics))
+      ];
+  }.
+
+  Definition of_ty :
+    OfTy.t (Ty.path "alloy_primitives::log::LogData").
+  Proof.
+    eapply OfTy.Make with (A := t).
+    now subst.
+  Defined.
+  Smpl Add unshelve eapply of_ty : of_ty.
+
+  Lemma of_value_with
+      topics topics'
+      data data' :
+    topics' = φ topics ->
+    data' = φ data ->
+    Value.StructRecord "alloy_primitives::log::LogData" [] [] [
+      ("data", data');
+      ("topics", topics')
+    ] = φ (Build_t topics data).
+  Proof.
+    intros.
+    now subst.
+  Qed.
+  Smpl Add unshelve eapply of_value_with : of_value.
+End LogData.
+
+Module Impl_LogData.
+  Definition Self : Set :=
+    LogData.t.
+
+  (* pub fn new(topics: Vec<B256>, data: Bytes) -> Option<Self> *)
+  Instance run_new (topics : Vec.t aliases.B256.t Global.t) (data : Bytes.t) :
+    Run.Trait log.Impl_alloy_primitives_log_LogData.new [] [] [φ topics; φ data]
+    (option Self).
+  Proof.
+    constructor.
+    run_symbolic.
+  Admitted.
+End Impl_LogData.
+Export Impl_LogData.
