CoqOfRust/revm/revm_interpreter/instructions/links/control.v
@@ -314,7 +314,7 @@ Proof.
   destruct Impl_Default_for_Bytes.run.
   destruct (Impl_Into_for_From_T.run Impl_From_Vec_u8_for_Bytes.run).
   run_symbolic.
-Admitted.
+Defined.
 
 (*
 pub fn ret<WIRE: InterpreterTypes, H: Host + ?Sized>(
